\documentclass[12pt,a4paper]{article}
\usepackage[utf8]{inputenc}
\usepackage{amsmath}
\usepackage{amssymb}
\usepackage{cite}
\usepackage{mathtools}
\usepackage{titling}
\usepackage[hidelinks]{hyperref}
\usepackage{csquotes}
\usepackage{MnSymbol}
\usepackage{wasysym}
%\usepackage[margin=1in, top= 1in, bottom=1in]{geometry}
\usepackage[font={it}, labelfont=bf]{caption}
\usepackage{graphicx}
\DeclareGraphicsExtensions{.pdf}
\graphicspath{ {../images/} }

\author{Reid McIlroy-Young}
\title{CMSC 25025 \\ Homework 1}
\date{April 6, 2017}

\newcommand{\s}[2]{\sum^{#2}_{#1}}
\newcommand{\func}[2]{#1\left(#2\right)}

\DeclareMathOperator*{\argmin}{argmin}

\renewcommand{\thesubsection}{\thesection.\alph{subsection}}

\begin{document}
\maketitle

\section{Statistical refresher}
\subsection{}

\begin{align*}
F(X) &= \int_{-\infty}^{X} f_x(t) dt\\
\Rightarrow f_x&= \frac{dF}{dX}
\end{align*}

\begin{align*}
X &= F^{-1}(U)\\
F(X) &= F(F^{-1}(U))\\
F(X) &= U\\
\Rightarrow X &\sim F
\end{align*}

\subsection{}

\begin{align}
X, Y \sim Uniform(0,1)\\
f_{X,Y}(x,y) &= 1
\end{align}

\begin{align*}
Z &= X - Y\\
F_Z(z) &= P(Z \leq z)\\
&= P(X - Y\leq z)\\
&= \begin{cases}
\int^{1 + z}_0\int^{1}_{y - z} dx dy & 1 \leq z \leq 0\\
1 - \int^{1}_{z}\int^{y - z}_{0} dx dy & 0 < z \leq -1\\
0 & else
\end{cases}\\
&= \begin{cases}
\int^{1 + z}_0 1 - y - z dy & 1 \leq z \leq 0\\
1 - \int^{1}_{z} y - z dx dy & 0 < z \leq -1\\
0 & else
\end{cases}\\
&= \begin{cases}
1 + z - \frac{(1+z)^2}{2} - z(1 + z) & 1 \leq z \leq 0\\
1 - (\frac{(1)^2}{2} - z - \frac{(z)^2}{2} + z^2) & 0 < z \leq -1\\
0 & else
\end{cases}\\
&= \begin{cases}
\frac{(z)^2}{2} + z + \frac{1}{2} & 1 \leq z \leq 0\\
- \frac{(z)^2}{2} + z + \frac{1}{2} & 0 < z \leq -1\\
0 & else
\end{cases}\\
\Rightarrow f_z(z) &= \begin{cases}
z + 1 & 1 \leq z \leq 0\\
- z + 1 & 0 < z \leq -1\\
0 & else
\end{cases}\\
\end{align*}

\begin{align*}
Z &= min\lbrace X, Y \rbrace\\
F_Z(z) &= P(Z \leq z)\\
&= P(min\lbrace X, Y \rbrace\leq z)\\
&= 1 - P(min\lbrace X, Y \rbrace\geq z)\\
&= 1 - P(X \geq z)P(Y \geq z)\\
&= 1 - (1 - z)(1 - z)\\
&= 2z - z^2
\end{align*}

\subsection{}
\begin{align}
x &\sim N(0, 1)\\
Y &= e^X\\
u^{-1}(Y) &= log(Y) \\
\frac{du^-1}{dY} &= \frac{1}{Y}\\
\Rightarrow f_Y(y) &= \frac{1}{y \sqrt{2\pi}} e^{\frac{log^2(y)}{2}}
\end{align}

\begin{align*}
\mathbf{E}(Y) &= \int^{\infty}_{-\infty} y \frac{1}{y \sqrt{2\pi}} e^{\frac{log^2(y)}{2}}dy\\
&= \int^{\infty}_{-\infty} \frac{1}{\sqrt{2\pi}} e^{\frac{log^2(y)}{2}}dy\\
&= e^{\frac{1}{2}}
\end{align*}

\begin{align*}
\mathbf{E}(Y^2) &= \int^{\infty}_{-\infty} y^2 \frac{1}{y \sqrt{2\pi}} e^{\frac{log^2(y)}{2}}dy\\
&= \int^{\infty}_{-\infty} \frac{y}{\sqrt{2\pi}} e^{\frac{log^2(y)}{2}}dy\\
&= e^{2}
\end{align*}

\begin{align*}
Var(Y) &= \mathbf{E}(Y^2) - [\mathbf{E}(Y)]^2\\
&= e^{2} - [e^{\frac{1}{2}}]^2\\
&= e^{2} - e
\end{align*}

\subsection{}
\begin{align*}
Var(Y) &= \mathbf{E}(Y^2) - [\mathbf{E}(Y)]^2\\
&= \mathbf{E}(\mathbf{E}[Y^2| X]) - [\mathbf{E}(\mathbf{E}[Y| X])]^2\\
&= \mathbf{E}(Var(Y|X) + [\mathbf{E}(Y | X)]^2) - [\mathbf{E}(\mathbf{E}[Y| X])]^2\\
&= \mathbf{E}(Var(Y|X)) + \mathbf{E}([\mathbf{E}(Y | X)]^2) - [\mathbf{E}(\mathbf{E}[Y| X])]^2\\
&= \mathbf{E}(Var(Y|X)) + Var(\mathbf{E}(Y|X))
\end{align*}

\section{Basic Regression}
\begin{align}
H &= X(X^T X)^{-1}X^T\\
\hat{\beta} &= (X^T X)^{-1}X^T\mathbf{y}\\
\end{align}

\subsection{}
\begin{align*}
H\textbf{y}&= (X(X^T X)^{-1}X^T)\textbf{y}\\
&=X((X^T X)^{-1}X^T\textbf{y})\\
 &= X\hat{\beta}
\end{align*}

\subsection{}
\begin{align*}
HX&= X(X^T X)^{-1}X^TX\\
&= XI\\
&=X
\end{align*}

\subsection{}
\begin{align*}
H^T&= (X(X^T X)^{-1}X^T)^T\\
&= {X^T}^T{(X^T X)^{-1}}^TX^T\\
&= X(X^T {X^T}^T)^{-1}X^T\\
&= X(X^T X)^{-1}X^T)\\
&= H
\end{align*}

\subsection{}
\begin{align*}
H^2&= (X(X^T X)^{-1}X^T)^2\\
&= (X(X^T X)^{-1}X^T)(X(X^T X)^{-1}X^T) \\
&= X(X^T X)^{-1}IX^T \\
&= (X(X^T X)^{-1}X^T)^2\\
&= H
\end{align*}
\subsection{}

\subsection{}
\begin{align*}
trace(H) &= trace(X(X^T X)^{-1}X^T)\\
&= trace((X^T X)^{-1}X^TX)\\
&= trace(I_d) \\
&= d = rank(X)\quad \because \text{H is a projection}
\end{align*}

\section{SVD}

\begin{align}
rank(X) &= r\\
X &= U\Sigma V^T\\
\Sigma_{ii} &= \sigma_i
U_i = \textbf{u}_i\\
V_i = \textbf{v}_i
\end{align}

\subsection{}

\begin{align*}
XX^T\textbf{u}_i &= U\Sigma V^T(U\Sigma V^T)^T\textbf{u}_i\\
&= U\Sigma V^TV\Sigma^T U^T\textbf{u}_i\\
&= U\Sigma\Sigma^T U^T\textbf{u}_i\\
&= U\Sigma^2 U^T\textbf{u}_i\\
&= \lambda \textbf{u}_i  \because \text{U is orthogonal } \exists \lambda\\
\lambda &= \sigma_i^2 \because \text{U is unitary } \exists \lambda
\end{align*}

\begin{align*}
X^TX\textbf{v}_i &= (U\Sigma V^T)^TU\Sigma V^T\textbf{v}_i\\
&= V\Sigma^T U^TU\Sigma V^T\textbf{v}_i\\
&= V\Sigma\Sigma^T V^T\textbf{v}_i\\
&= V\Sigma^2 V^T\textbf{v}_i\\
&= \lambda \textbf{v}_i  \because \text{V is orthogonal } \exists \lambda\\
\lambda &= \sigma_i^2 \because \text{U is unitary } \exists \lambda
\end{align*}

\subsection{}

\begin{align*}
X \textbf{u}_i   &= U\Sigma V^T \textbf{u}_i\\
\end{align*}

\subsection{}
\subsection{}
\subsection{}

\begin{align*}
H &= X(X^TX)^{-1}X^T\\
&= U\Sigma V^T ((U\Sigma V^T)^TU\Sigma V^T)^{-1}(U\Sigma V^T)^T\\
&= U\Sigma V^T (V\Sigma^TU^TU\Sigma V^T)^{-1}V\Sigma^TU^T\\
&= U\Sigma V^T (V\Sigma^2 V^T)^{-1}V\Sigma^TU^T\\
&= U\Sigma V^T V\Sigma^{-2} V^TV\Sigma^TU^T\\
&= U\Sigma \Sigma^{-2}\Sigma^TU^T\\
&= UU^T\\
\end{align*}


\end{document}